Add intro

new-semantics/coq/cfa/Defs.v
@@ -1,33 +1,135 @@
 From Basics Require Import Basics.
 From With_events Require Import Syntax.
+From With_events Require Import Defs.
 From With_events Require Import EnvSemantics.
 From CFA Require Import Syntax.
 
-Fixpoint is_repr {var lbl} (t : @tm var lbl) (g : lbl -> ltm) :=
-  match t with
-  | tm_var p x =>
-    g p = ltm_var x
-  | tm_lam p x t =>
-    g p = ltm_lam x (get_lbl t) /\ is_repr t g
-  | tm_app p t1 t2 =>
-    g p = ltm_app (get_lbl t1) (get_lbl t2) /\ is_repr t1 g /\ is_repr t2 g
-  | tm_link p t1 t2 =>
-    g p = ltm_link (get_lbl t1) (get_lbl t2) /\ is_repr t1 g /\ is_repr t2 g
-  | tm_mt p =>
-    g p = ltm_mt
-  | tm_bind p x t1 t2 =>
-    g p = ltm_bind x (get_lbl t1) (get_lbl t2) /\ is_repr t1 g /\ is_repr t2 g
-  end
-.
+Section defs.
+  Context {var lbl : Type}.
 
-Definition geq {var lbl} (v1 v2 : @abs_val var lbl) :=
-  match v1, v2 with
-  | ((σ1, E1), λ1), ((σ2, E2), λ2) =>
-    (forall x p, In p (σ2 x) -> In p (σ1 x)) /\
-    (forall E, In E E2 -> In E E1) /\
-    (forall λ, In λ λ2 -> In λ λ1)
-  end.
+  Fixpoint is_repr (t : @tm var lbl) (g : lbl -> ltm) :=
+    match t with
+    | tm_var p x =>
+      g p = ltm_var x
+    | tm_lam p x t =>
+      g p = ltm_lam x (get_lbl t) /\ is_repr t g
+    | tm_app p t1 t2 =>
+      g p = ltm_app (get_lbl t1) (get_lbl t2) /\ is_repr t1 g /\ is_repr t2 g
+    | tm_link p t1 t2 =>
+      g p = ltm_link (get_lbl t1) (get_lbl t2) /\ is_repr t1 g /\ is_repr t2 g
+    | tm_mt p =>
+      g p = ltm_mt
+    | tm_bind p x t1 t2 =>
+      g p = ltm_bind x (get_lbl t1) (get_lbl t2) /\ is_repr t1 g /\ is_repr t2 g
+    end
+  .
+
+  Definition geq (v1 v2 : @abs_val var lbl) :=
+    (forall x p, In p (v2.(_σ).(_β) x) -> In p (v1.(_σ).(_β) x)) /\
+    (forall E, In E v2.(_σ).(_E) -> In E v1.(_σ).(_E)) /\
+    (forall λ, In λ v2.(_λ) -> In λ v1.(_λ))
+  .
+
+  Definition aval_of_aenv {var lbl} (σ : @abs_env var lbl) :=
+    {| _σ := σ; _λ := [] |}.
+
+  #[local] Coercion aval_of_aenv : abs_env >-> abs_val.
+  #[local] Coercion vl_ev : vnt >-> vl.
+  #[local] Coercion vl_exp : nv >-> vl.
+  #[local] Coercion wvl_v : vl >-> wvl.
+
+  Inductive conc {loc} (t : @abs_sem var lbl) (v : abs_val) : wvl var lbl loc _ -> Prop :=
+  | conc_nil
+  : conc t v nv_mt
+  | conc_enil (E : vnt _ _ _ _)
+    (VNT : conc t v E)
+  : conc t v (nv_ev E)
+  | cons_floc x ℓ p (σ : nv _ _ _ _)
+    (LOC : In p (v.(_σ).(_β) x))
+    (ENV : conc t v σ)
+  : conc t v (nv_floc x (ℓ, p) σ)
+  | conc_wval x w p (σ : nv _ _ _ _)
+    (LOC : In p (v.(_σ).(_β) x))
+    (VAL : conc t (t p).(_o) w)
+    (ENV : conc t v σ)
+  : conc t v (nv_bval x w σ)
+  | conc_clos x e p (σ : nv _ _ _ _)
+    (LAM : In (lv_fn x (get_lbl e), p) v.(_λ))
+    (ENV : conc t (t p).(_i) σ)
+  : conc t v (vl_clos (v_fn x e) σ)
+  | conc_rec L p v'
+    (VAL : forall ℓ (nIN : ~ In ℓ L), conc t v (open_loc_vl 0 (ℓ, p) v'))
+    (ROLL : forall ℓ (nIN : ~ In ℓ L), conc t (t p).(_o) (open_loc_vl 0 (ℓ, p) v'))
+  : conc t v (wvl_recv p v')
+  | conc_Init
+    (VNT : In AInit v.(_σ).(_E))
+  : conc t v Init
+  | conc_Read p (E : vnt _ _ _ _) x
+    (VNT : In (ARead p x) v.(_σ).(_E))
+    (ENV : conc t (t p).(_i) E)
+  : conc t v (Read E x)
+  | conc_Call p1 p2 (E : vnt _ _ _ _) (v' : vl _ _ _ _)
+    (VNT : In (ACall p1 p2) v.(_σ).(_E))
+    (FN : conc t (t p1).(_o) E)
+    (ARG : conc t (t p2).(_o) v')
+  : conc t v (Call E v')
+  .
+
+  Ltac conc_lc_tac := 
+    repeat match goal with
+    | _ => solve [auto]
+    | H : wvalue (_ _) |- _ => inv H
+    | H : env (_ _) |- _ => inv H
+    | H : value (_ _) |- _ => inv H
+    | H : event (_ _) |- _ => inv H
+    | L : list _ |- _ => instantiate (1 := L)
+    end.
+
+  Lemma conc_lc {loc} t v w (CONC : @conc loc t v w) : wvalue w.
+  Proof.
+    induction CONC;
+    repeat econstructor; des;
+    conc_lc_tac; ii.
+    exploit H; eauto. ii. conc_lc_tac.
+  Qed.
+
+  (* monotonicity of concretization in v *)
+  Lemma conc_mon_fst {loc} t v w (CONC : @conc loc t v w) v' (GEQ : geq v' v) :
+    conc t v' w.
+  Proof.
+    induction CONC; ii; ss;
+    repeat match goal with
+    | H : ?P, IH : ?P -> _ |- _ => specialize (IH H)
+    end; econstructor; eauto;
+    match goal with
+    | GE : geq _ _ |- _ =>
+      destruct GE as (A & B & C); eauto
+    end.
+  Qed.
+
+  (* monotonicity of concretization in t *)
+  Lemma conc_mon_snd {loc} t v w (CONC : @conc loc t v w) t'
+    (GEQ : forall p, geq (t' p).(_i) (t p).(_i) /\ geq (t' p).(_o) (t p).(_o)) :
+      conc t' v w.
+  Proof.
+    induction CONC; ii; ss;
+    econstructor; eauto;
+    ii; eapply conc_mon_fst;
+    try_all; eauto; eapply GEQ.
+  Qed.
+End defs.
 
 Notation "v1 '⊒' v2" := (geq v1 v2)
   (at level 100, v2 at next level, right associativity).
+Notation "t v '⪰' w" := (conc t v w)
+  (at level 100, v at next level, w at next level, right associativity).
+
+Ltac des_geq :=
+  match goal with
+  | H : geq _ _ |- _ =>
+    let geσ := fresh "geσ" in
+    let geE := fresh "geE" in
+    let geλ := fresh "geλ" in
+    destruct H as (geσ & geE & geλ)
+  end.
 
