new-semantics/coq/cfa/Syntax.v
@@ -1,3 +1,5 @@
+Set Primitive Projections.
+
 Section syntax.
   Context {var lbl : Type}.
 
@@ -10,21 +12,38 @@ Section syntax.
   | ltm_mt
   | ltm_bind (x : var) (p1 p2 : lbl)
   .
-  
+
   Variant lval :=
   | lv_fn (x : var) (p : lbl)
   .
-  
+
   Variant avnt :=
   | AInit
   | ARead (p : lbl) (x : var)
   | ACall (p1 p2 : lbl)
   .
- 
-  Definition abs_env : Type := (var -> list lbl) * list avnt.
- 
-  Definition abs_val : Type := abs_env * list (lval * lbl).
- 
-  Definition abs_sem : Type := lbl -> (abs_env * abs_val).
+
+  Record abs_env := mkEnv {
+    _β : var -> list lbl;
+    _E : list avnt;
+  }.
+
+  Definition aenv_bot := {| _β := fun _ => nil; _E := nil |}.
+
+  Record abs_val := mkVal {
+    _σ : abs_env;
+    _λ : list (lval * lbl);
+  }.
+
+  Definition aval_bot := {| _σ := aenv_bot; _λ := nil |}.
+
+  Record io := mkIO {
+    _i : abs_env;
+    _o : abs_val;
+  }.
+
+  Definition abs_sem : Type := lbl -> io.
+
+  Definition asem_bot : abs_sem := fun _ => {| _i := aenv_bot; _o := aval_bot |}.
 End syntax.
 
